dimsum_examples/compiler/ssa.v
@@ -134,9 +134,9 @@ Proof.
   - apply: IHes'1; [done|done|] => /= ??.
     apply: IHes'2; [done|rewrite pass_state;naive_solver lia|] => /= ??.
     tstep_s => ??. tstep_i. split!. by apply tsim_mono_b_false.
-  - apply: IHes'; try done. intros => /=.
+  - apply: IHes'; [done..|]. move => ? v'/=.
     destruct v' eqn:?; [| tstep_s; done..].
-    destruct (decide (z>0)) eqn:?.
+    destruct (decide (z > 0)) eqn:?.
     2:{ tstep_s. split! => *; [apply heap_fresh_is_fresh|]. done. }
     tstep_i => *. destruct!. split!.
     tstep_s => *. split! => *; [done|]. by apply tsim_mono_b_false.
